Dodal komentarje v imp_safety.lean

imp_safety.lean
@@ -1,5 +1,7 @@
--- Syntax
+-- ==================== Syntax ====================
+
 def loc := string
+
 
 inductive aexp : Type
 | Lookup : loc -> aexp
@@ -8,11 +10,13 @@ inductive aexp : Type
 | Minus : aexp -> aexp -> aexp
 | Times : aexp -> aexp -> aexp
 
+
 inductive bexp : Type
 | Bool : bool -> bexp
 | Equal : aexp -> aexp -> bexp
 | Less : aexp -> aexp -> bexp
 | Greater : aexp -> aexp -> bexp
+
 
 inductive cmd : Type
 | Assign : loc -> aexp -> cmd
@@ -21,7 +25,7 @@ inductive cmd : Type
 | Skip : cmd
 | WhileDo : bexp -> cmd -> cmd
 
--- Example 'fact.imp' in LEAN notation.
+-- ================== Example 'fact.imp' in LEAN notation. ==================
 
 def fact : cmd :=
   cmd.Seq
@@ -38,24 +42,26 @@ def fact : cmd :=
         (cmd.Assign "n"
           (aexp.Minus (aexp.Lookup "n") (aexp.Int 1)) ) ) )
 
--- State
+-- ==================== Environment ====================
 
 inductive env : Type
 | Nil : env
 | Cons : loc -> int -> env -> env
 
+
 inductive lookup : loc -> env -> int -> Prop
 | Find {loc i E} : 
     lookup loc (env.Cons loc i E) i 
 | Search {loc loc' i' E' i} : 
-    loc'≠loc -> lookup loc E' i -> 
+    loc≠loc' -> lookup loc E' i -> 
     lookup loc (env.Cons loc' i' E') i
 
--- Operational Semantics
+-- ==================== Operational Semantics ====================
 
 inductive aeval : env -> aexp -> int -> Prop
 | Lookup {E loc i} :
-    lookup loc E i -> aeval E (aexp.Lookup loc) i
+    lookup loc E i -> 
+    aeval E (aexp.Lookup loc) i
 | Int {E i} :
     aeval E (aexp.Int i) i
 | Plus {E a1 a2 i1 i2} :
@@ -68,6 +74,8 @@ inductive aeval : env -> aexp -> int -> Prop
     aeval E a1 i1 -> aeval E a2 i2 ->
     aeval E (aexp.Times a1 a2) (i1 * i2)
 
+
+-- Lean works best with '<' and '≤' so we use them to encode '>' and '≥'.
 inductive beval : env -> bexp -> bool -> Prop
 | Bool {E b} :
     beval E (bexp.Bool b) b
@@ -89,6 +97,7 @@ inductive beval : env -> bexp -> bool -> Prop
 | Greater_f {E a1 a2 i1 i2}:
     aeval E a1 i1 -> aeval E a2 i2 -> i1 ≤ i2 ->
     beval E (bexp.Greater a1 a2) false
+
 
 inductive ceval : env -> cmd -> env -> Prop
 | Assign {loc a i E} :
@@ -113,22 +122,25 @@ inductive ceval : env -> cmd -> env -> Prop
     beval E b false -> 
     ceval E (cmd.WhileDo b c) E
 
--- Safety
+-- ==================== Safety ====================
 
+-- Contains all the names of already assigned locations.
 inductive locs : Type
 | Nil : locs
 | Cons : loc -> locs -> locs
 
-inductive safe_in : locs -> loc -> Prop
+
+inductive loc_safe : loc -> locs -> Prop
 | Find {loc L} : 
-    safe_in (locs.Cons loc L) loc 
+    loc_safe loc (locs.Cons loc L) 
 | Search {loc loc' L} : 
-    loc'≠loc -> safe_in L loc -> 
-    safe_in (locs.Cons loc' L) loc 
+    loc'≠loc -> loc_safe loc L -> 
+    loc_safe loc (locs.Cons loc' L)
+
 
 inductive asafe : locs -> aexp -> Prop
 | Lookup {L loc}:
-    safe_in L loc -> asafe L (aexp.Lookup loc)
+    loc_safe loc L -> asafe L (aexp.Lookup loc)
 | Int {L i}:
     asafe L (aexp.Int i)
 | Plus {L a1 a2} :
@@ -140,6 +152,7 @@ inductive asafe : locs -> aexp -> Prop
 | Times {L a1 a2} :
     asafe L a1 -> asafe L a2 ->
     asafe L (aexp.Times a1 a2)
+
 
 inductive bsafe : locs -> bexp -> Prop
 | Bool {L b} :
@@ -154,13 +167,14 @@ inductive bsafe : locs -> bexp -> Prop
     asafe L a1 -> asafe L a2 ->
     bsafe L (bexp.Greater a1 a2)
 
+
 inductive csafe : locs -> cmd -> locs -> Prop
 | Assign {L loc a} :
     asafe L a ->
     csafe L (cmd.Assign loc a) (locs.Cons loc L)
 -- | IfThenElse {L b c1 c2} :
 --     bsafe L b -> csafe L c1 L' -> csafe L c2 L'' ->
---     ???  
+-- Note: This part requires a definition of locs intersection. 
 | Seq {L c1 L' c2 L''} :
     csafe L c1 L' -> csafe L' c2 L'' ->
     csafe L (cmd.Seq c1 c2) L''
@@ -170,119 +184,154 @@ inductive csafe : locs -> cmd -> locs -> Prop
     bsafe L b -> csafe L c L' ->
     csafe L (cmd.WhileDo b c) L'
 
--- Checks for envirnoment safety with regard to locations
-inductive env_safe : env -> locs -> Prop
+-- ==================== Auxiliary safety for lookup ====================
+
+-- Proves that the given environment maps all the required locations.
+inductive env_maps : env -> locs -> Prop
 | Nil {E} :
-    env_safe E locs.Nil
+    env_maps E locs.Nil
 | Cons {loc E L} :
-    env_safe E L -> (∃i, lookup loc E i) ->
-    env_safe E (locs.Cons loc L)
+    env_maps E L -> (∃i, lookup loc E i) ->
+    env_maps E (locs.Cons loc L)
 
-theorem env_safe_weaken {E L loc i}:
-  env_safe E L -> env_safe (env.Cons loc i E) L
+
+-- Increasing the environment does not break its safety.
+theorem env_maps_weaken {E L loc i}:
+  env_maps E L -> env_maps (env.Cons loc i E) L
 :=
 begin
-  intro es, induction es,
-  apply env_safe.Nil,
-  apply env_safe.Cons, assumption,
-  cases string.has_decidable_eq loc es_loc,
-  { cases es_a_1 with i', existsi i',
+  intro es, induction es with E' loc' E' L' maps finds ih,
+  apply env_maps.Nil,
+  apply env_maps.Cons, assumption,
+  -- we compare the the strings to know which lookup result is correct
+  cases string.has_decidable_eq loc' loc with neq eq,
+  { cases finds with i', existsi i',
     apply lookup.Search, assumption, assumption, },
-  subst h, existsi i, apply lookup.Find,
+  existsi i, subst eq, apply lookup.Find,
 end
 
+
+-- If the location is safe in the same specification as the environment
+-- then we are guaranteed to look up a value
 theorem safe_lookup {L E loc}:
-  safe_in L loc -> env_safe E L -> ∃ (i:int), lookup loc E i
+  loc_safe loc L -> env_maps E L -> ∃ (i:int), lookup loc E i
 :=
 begin
-  intros sloc es, induction es,
+  intros sloc es, 
+  induction es with E' loc' E' L' maps finds ih,
   { cases sloc, },
-  cases sloc, assumption, apply es_ih, assumption,
+  cases sloc, assumption, apply ih, assumption,
 end
 
--- Safety theorems
+-- ==================== Safety theorems ====================
+
 theorem asafety {L E a}:
-  asafe L a -> env_safe E L -> ∃ (i:int), aeval E a i
+  asafe L a -> env_maps E L -> ∃ (i:int), aeval E a i
 :=
 begin
   intros s es,
   induction s,
-  { cases safe_lookup s_a es,
-    existsi w, apply aeval.Lookup, assumption, },
-  { existsi s_i, apply aeval.Int, },
-  { cases s_ih_a es with i1,
-    cases s_ih_a_1 es with i2,
-    existsi (i1+i2), apply aeval.Plus, assumption, assumption },
-  { cases s_ih_a es with i1,
-    cases s_ih_a_1 es with i2,
-    existsi (i1-i2), apply aeval.Minus, assumption, assumption },
-  { cases s_ih_a es with i1,
-    cases s_ih_a_1 es with i2,
-    existsi (i1*i2), apply aeval.Times, assumption, assumption },
+  case asafe.Lookup
+    { cases safe_lookup s_a es,
+      existsi w, apply aeval.Lookup, assumption, },
+  case asafe.Int
+    { existsi s_i, apply aeval.Int, },
+  case asafe.Plus
+    { cases s_ih_a es with i1,
+      cases s_ih_a_1 es with i2,
+      existsi (i1+i2), apply aeval.Plus, 
+      assumption, assumption },
+  case asafe.Minus
+    { cases s_ih_a es with i1,
+      cases s_ih_a_1 es with i2,
+      existsi (i1-i2), apply aeval.Minus, 
+      assumption, assumption },
+  case asafe.Times
+    { cases s_ih_a es with i1,
+      cases s_ih_a_1 es with i2,
+      existsi (i1*i2), apply aeval.Times, 
+      assumption, assumption },
 end
+
 
 theorem bsafety {L E b}:
-  bsafe L b -> env_safe E L -> ∃ (v:bool), beval E b v
+  bsafe L b -> env_maps E L -> ∃ (v:bool), beval E b v
 :=
 begin
   intros s es,
   induction s,
-  { existsi s_b, apply beval.Bool, },
-  { cases asafety s_a es with i1,
-    cases asafety s_a_1 es with i2,
-    cases int.decidable_eq i1 i2 with eq,
-    { existsi (false:bool), apply beval.Equal_f,
-      assumption, assumption, assumption,},
-    { existsi (true:bool), apply beval.Equal_t,
-      assumption, assumption, assumption,}, },
-  { cases asafety s_a es with i1,
-    cases asafety s_a_1 es with i2,
-    cases int.decidable_lt i1 i2 with eq,
-    { existsi (false:bool), apply beval.Less_f,
-      assumption, assumption, assumption,},
-    { existsi (true:bool), apply beval.Less_t,
-      assumption, assumption, assumption,}, },
-  { cases asafety s_a es with i1,
-    cases asafety s_a_1 es with i2,
-    cases int.decidable_le i1 i2 with eq,
-    { existsi (true:bool), apply beval.Greater_t,
-      assumption, assumption, assumption,},
-    { existsi (false:bool), apply beval.Greater_f,
-      assumption, assumption, assumption,}, },
+  case bsafe.Bool
+    { existsi s_b, apply beval.Bool, },
+  case bsafe.Equal
+    { cases asafety s_a es with i1,
+      cases asafety s_a_1 es with i2,
+      cases int.decidable_eq i1 i2 with neq eq,
+      -- i1 ≠ i2
+      { existsi (false:bool), apply beval.Equal_f,
+        assumption, assumption, assumption,},
+      -- i1 = i2
+      { existsi (true:bool), apply beval.Equal_t,
+        assumption, assumption, assumption,}, },
+  case bsafe.Less
+    { cases asafety s_a es with i1,
+      cases asafety s_a_1 es with i2,
+      cases int.decidable_lt i1 i2 with neq eq,
+      -- i1 ≰ i2
+      { existsi (false:bool), apply beval.Less_f,
+        assumption, assumption, assumption,},
+      -- i1 < i2
+      { existsi (true:bool), apply beval.Less_t,
+        assumption, assumption, assumption,}, },
+  case bsafe.Greater
+    { cases asafety s_a es with i1,
+      cases asafety s_a_1 es with i2,
+      cases int.decidable_le i1 i2 with neq eq,
+      -- i > i2
+      { existsi (true:bool), apply beval.Greater_t,
+        assumption, assumption, assumption,},
+      -- i ≱ i2
+      { existsi (false:bool), apply beval.Greater_f,
+        assumption, assumption, assumption,}, },
 end
 
+
 theorem csafety {L L' E c }:
-  csafe L c L' -> env_safe E L -> 
-  ∃ (E':env), ceval E c E' ∧ env_safe E' L'
+  csafe L c L' -> env_maps E L -> ∃ (E':env), ceval E c E' ∧ env_maps E' L'
 :=
 begin
-  intros safe, revert E,
-  induction safe; intros E es,
-  { cases asafety safe_a_1 es with i,
-    existsi (env.Cons safe_loc i E),
-    constructor,
-    { apply ceval.Assign, assumption, },
-    apply env_safe.Cons,
-    { apply env_safe_weaken, assumption, },
-    existsi i, apply lookup.Find, },
-  { cases (safe_ih_a es) with E',
-    destruct h, intros c1safe es',
-    cases (safe_ih_a_1 es') with E'',
-    destruct h_1, intros c2safe es'',
-    existsi E'', constructor,
-    { apply ceval.Seq, assumption, assumption, },
-    assumption, },
-  { existsi E, constructor, apply ceval.Skip, assumption, },
-  { cases (safe_ih es) with E',
-    destruct h, intros csafe es',
-    cases bsafety safe_a es,
-    cases w,
-    { existsi E, constructor,
-      apply ceval.WhileDo_f,
-      assumption, sorry, }, -- subset?
-    { existsi E', constructor,
-      apply ceval.WhileDo_t,
-      assumption, assumption, sorry, sorry, } 
-      -- need to recursively check stuff?
-     },
+  intros s, revert E,
+  induction s; intros E es,
+  case csafe.Assign
+    { cases asafety s_a_1 es with i,
+      existsi (env.Cons s_loc i E),
+      constructor,
+      { apply ceval.Assign, assumption, },
+      apply env_maps.Cons,
+      { apply env_maps_weaken, assumption, },
+      existsi i, apply lookup.Find, },
+  case csafe.Seq
+    { cases (s_ih_a es) with E',
+      destruct h, intros c1s es',
+      cases (s_ih_a_1 es') with E'',
+      destruct h_1, intros c2s es'',
+      existsi E'', constructor,
+      { apply ceval.Seq, assumption, assumption, },
+      assumption, },
+  case csafe.Skip
+    { existsi E, constructor, apply ceval.Skip, assumption, },
+  case csafe.WhileDo
+    { 
+      -- this part can't really be done in big step semantics
+      cases (s_ih es) with E',
+      destruct h, intros csafe es',
+      cases bsafety s_a es,
+      cases w,
+      { existsi E, constructor,
+        apply ceval.WhileDo_f,
+        assumption, sorry, },
+      { existsi E', constructor,
+        apply ceval.WhileDo_t,
+        assumption, assumption, 
+        sorry, sorry, } 
+      },
 end
